Stack/StackLanguage.thy
@@ -8,25 +8,27 @@ datatype stack_instruction =
 
 type_synonym stack_program = "code_label \<rightharpoonup> stack_instruction list \<times> code_label"
 
-type_synonym stack_state = "int list \<times> stack_instruction list \<times> code_label \<times> output" 
+datatype stack_value =
+  IntV int
+| Bool bool
+
+type_synonym stack_state = "stack_value list \<times> stack_instruction list \<times> code_label \<times> output" 
   (* \<sigma>, \<pi>, s, \<omega> *)
 
 fun eval_stack :: "stack_program \<Rightarrow> stack_state \<Rightarrow> stack_state option" where
   "eval_stack \<Pi> (\<sigma>, [], s, \<omega>) = (case \<Pi> s of
       Some (\<pi>, s') \<Rightarrow> Some (\<sigma>, \<pi>, s', \<omega>)
     | None \<Rightarrow> None)"
-| "eval_stack \<Pi> (i1 # i2 # \<sigma>, Add # \<pi>, s, \<omega>) = Some ((i2 + i1) # \<sigma>, \<pi>, s, \<omega>)"
-| "eval_stack \<Pi> (i1 # i2 # \<sigma>, Sub # \<pi>, s, \<omega>) = Some ((i2 - i1) # \<sigma>, \<pi>, s, \<omega>)"
-| "eval_stack \<Pi> (i1 # \<sigma>, Neg # \<pi>, s, \<omega>) = Some ((-i1) # \<sigma>, \<pi>, s, \<omega>)"
-| "eval_stack \<Pi> (i1 # i2 # \<sigma>, Eq # \<pi>, s, \<omega>) = Some (unboolify (i2 = i1) # \<sigma>, \<pi>, s, \<omega>)"
-| "eval_stack \<Pi> (i1 # i2 # \<sigma>, Gt # \<pi>, s, \<omega>) = Some (unboolify (i2 > i1) # \<sigma>, \<pi>, s, \<omega>)"
-| "eval_stack \<Pi> (i1 # i2 # \<sigma>, Lt # \<pi>, s, \<omega>) = Some (unboolify (i2 < i1) # \<sigma>, \<pi>, s, \<omega>)"
-| "eval_stack \<Pi> (i1 # i2 # \<sigma>, And # \<pi>, s, \<omega>) = 
-    Some (unboolify (boolify i2 \<and> boolify i1) # \<sigma>, \<pi>, s, \<omega>)"
-| "eval_stack \<Pi> (i1 # i2 # \<sigma>, Or # \<pi>, s, \<omega>) = 
-    Some (unboolify (boolify i2 \<or> boolify i1) # \<sigma>, \<pi>, s, \<omega>)"
-| "eval_stack \<Pi> (i1 # \<sigma>, Not # \<pi>, s, \<omega>) = Some (unboolify (\<not> boolify i1) # \<sigma>, \<pi>, s, \<omega>)"
-| "eval_stack \<Pi> (i1 # \<sigma>, Print # \<pi>, s, \<omega>) = Some (\<sigma>, \<pi>, s, i1 # \<omega>)"
+| "eval_stack \<Pi> (IntV i1 # IntV i2 # \<sigma>, Add # \<pi>, s, \<omega>) = Some (IntV (i2 + i1) # \<sigma>, \<pi>, s, \<omega>)"
+| "eval_stack \<Pi> (IntV i1 # IntV i2 # \<sigma>, Sub # \<pi>, s, \<omega>) = Some (IntV (i2 - i1) # \<sigma>, \<pi>, s, \<omega>)"
+| "eval_stack \<Pi> (IntV i1 # \<sigma>, Neg # \<pi>, s, \<omega>) = Some (IntV (-i1) # \<sigma>, \<pi>, s, \<omega>)"
+| "eval_stack \<Pi> (IntV i1 # IntV i2 # \<sigma>, Eq # \<pi>, s, \<omega>) = Some (Bool (i2 = i1) # \<sigma>, \<pi>, s, \<omega>)"
+| "eval_stack \<Pi> (IntV i1 # IntV i2 # \<sigma>, Gt # \<pi>, s, \<omega>) = Some (Bool (i2 > i1) # \<sigma>, \<pi>, s, \<omega>)"
+| "eval_stack \<Pi> (IntV i1 # IntV i2 # \<sigma>, Lt # \<pi>, s, \<omega>) = Some (Bool (i2 < i1) # \<sigma>, \<pi>, s, \<omega>)"
+| "eval_stack \<Pi> (Bool i1 # Bool i2 # \<sigma>, And # \<pi>, s, \<omega>) = Some (Bool (i2 \<and> i1) # \<sigma>, \<pi>, s, \<omega>)"
+| "eval_stack \<Pi> (Bool i1 # Bool i2 # \<sigma>, Or # \<pi>, s, \<omega>) = Some (Bool (i2 \<or> i1) # \<sigma>, \<pi>, s, \<omega>)"
+| "eval_stack \<Pi> (Bool i1 # \<sigma>, Not # \<pi>, s, \<omega>) = Some (Bool (\<not> i1) # \<sigma>, \<pi>, s, \<omega>)"
+| "eval_stack \<Pi> (IntV i1 # \<sigma>, Print # \<pi>, s, \<omega>) = Some (\<sigma>, \<pi>, s, i1 # \<omega>)"
 | "eval_stack \<Pi> \<Sigma> = None"
 
 fun stack_output :: "stack_state \<Rightarrow> output" where
