TotalCorrectness.thy
@@ -3,29 +3,32 @@ imports
   "LinearAssembly/AssemblyToMachine" 
   "Assembly/Linearization" 
   "BranchingAssembly/Debranching" 
-  "Stack/StackToAssembly"
+  "FlatStack/StackToAssembly"
+  "Stack/Flattening"
 begin
 
 definition state_convert :: "stack_program \<Rightarrow> stack_state \<Rightarrow> machine_state set" where
   "state_convert \<Pi> \<Sigma>\<^sub>S = { \<Sigma>\<^sub>M | \<Sigma>\<^sub>B \<Sigma>\<^sub>M. 
-    \<Sigma>\<^sub>B \<in> StackToAssembly.state_convert \<Sigma>\<^sub>S \<and> 
+    \<Sigma>\<^sub>B \<in> StackToAssembly.state_convert (Flattening.state_convert \<Sigma>\<^sub>S) \<and> 
       \<Sigma>\<^sub>M \<in> AssemblyToMachine.state_convert
-        (linearize (debranch (StackToAssembly.program_convert \<Pi>))) 
+        (linearize (debranch (StackToAssembly.program_convert (flatten \<Pi>)))) 
           (Linearization.state_convert 
-            (Debranching.state_convert (dom (StackToAssembly.program_convert \<Pi>)) \<Sigma>\<^sub>B)) }"
+            (Debranching.state_convert (dom (StackToAssembly.program_convert (flatten \<Pi>))) \<Sigma>\<^sub>B)) }"
 
 definition program_convert :: "stack_program \<Rightarrow> machine_program" where
-  "program_convert \<Pi> =
-    AssemblyToMachine.program_convert (linearize (debranch (StackToAssembly.program_convert \<Pi>)))"
+  "program_convert = 
+    AssemblyToMachine.program_convert o linearize o 
+      debranch o StackToAssembly.program_convert o flatten"
 
 theorem output_equivalence: "\<Sigma>\<^sub>M \<in> state_convert \<Pi> \<Sigma>\<^sub>S \<Longrightarrow> machine_output \<Sigma>\<^sub>M = stack_output \<Sigma>\<^sub>S"
   proof -
-    let ?\<Pi>\<^sub>B = "StackToAssembly.program_convert \<Pi>"
+    let ?\<Pi>\<^sub>B = "StackToAssembly.program_convert (flatten \<Pi>)"
     let ?\<Pi>\<^sub>A = "linearize (debranch ?\<Pi>\<^sub>B)"
     assume "\<Sigma>\<^sub>M \<in> state_convert \<Pi> \<Sigma>\<^sub>S"
-    with state_convert_def obtain \<Sigma>\<^sub>B where B: "\<Sigma>\<^sub>B \<in> StackToAssembly.state_convert \<Sigma>\<^sub>S \<and> 
-      \<Sigma>\<^sub>M \<in> AssemblyToMachine.state_convert ?\<Pi>\<^sub>A (Linearization.state_convert 
-        (Debranching.state_convert (dom ?\<Pi>\<^sub>B) \<Sigma>\<^sub>B))" by blast
+    with state_convert_def obtain \<Sigma>\<^sub>B where B: "
+      \<Sigma>\<^sub>B \<in> StackToAssembly.state_convert (Flattening.state_convert \<Sigma>\<^sub>S) \<and> 
+        \<Sigma>\<^sub>M \<in> AssemblyToMachine.state_convert ?\<Pi>\<^sub>A (Linearization.state_convert 
+          (Debranching.state_convert (dom ?\<Pi>\<^sub>B) \<Sigma>\<^sub>B))" by blast
     thus ?thesis by auto
   qed
 
@@ -34,20 +37,23 @@ theorem total_correctness: "finite (dom \<Pi>) \<Longrightarrow> iterate (eval_s
     \<exists>\<Sigma>\<^sub>M'. \<Sigma>\<^sub>M' \<in> state_convert \<Pi> \<Sigma>\<^sub>S' \<and> iterate (eval_machine (program_convert \<Pi>)) \<Sigma>\<^sub>M \<Sigma>\<^sub>M'"
   proof -
     assume D: "finite (dom \<Pi>)"
-    hence DA: "finite (dom (StackToAssembly.program_convert \<Pi>))" by simp
-    hence DF: "finite (dom (debranch (StackToAssembly.program_convert \<Pi>)))" by simp
-    hence DL: "domain_distinct (linearize (debranch (StackToAssembly.program_convert \<Pi>)))" by simp
+    hence DA: "finite (dom (StackToAssembly.program_convert (flatten \<Pi>)))" by simp
+    hence DF: "finite (dom (debranch (StackToAssembly.program_convert (flatten \<Pi>))))" by simp
+    hence DL: "domain_distinct (linearize (debranch (StackToAssembly.program_convert (flatten \<Pi>))))" 
+      by simp
     assume ES: "iterate (eval_stack \<Pi>) \<Sigma>\<^sub>S \<Sigma>\<^sub>S'"
-    let ?\<Pi>\<^sub>B = "StackToAssembly.program_convert \<Pi>"
+    let ?\<Pi>\<^sub>B = "StackToAssembly.program_convert (flatten \<Pi>)"
     let ?\<Pi>\<^sub>A = "debranch ?\<Pi>\<^sub>B"
     let ?\<Pi>\<^sub>M = "AssemblyToMachine.program_convert (linearize ?\<Pi>\<^sub>A)"
     assume "\<Sigma>\<^sub>M \<in> state_convert \<Pi> \<Sigma>\<^sub>S"
-    with state_convert_def obtain \<Sigma>\<^sub>B where B: "\<Sigma>\<^sub>B \<in> StackToAssembly.state_convert \<Sigma>\<^sub>S \<and> 
-      \<Sigma>\<^sub>M \<in> AssemblyToMachine.state_convert (linearize ?\<Pi>\<^sub>A) 
-        (Linearization.state_convert (Debranching.state_convert (dom ?\<Pi>\<^sub>B) \<Sigma>\<^sub>B))" 
+    with state_convert_def obtain \<Sigma>\<^sub>B where B: 
+      "\<Sigma>\<^sub>B \<in> StackToAssembly.state_convert (Flattening.state_convert \<Sigma>\<^sub>S) \<and> 
+        \<Sigma>\<^sub>M \<in> AssemblyToMachine.state_convert (linearize ?\<Pi>\<^sub>A) 
+          (Linearization.state_convert (Debranching.state_convert (dom ?\<Pi>\<^sub>B) \<Sigma>\<^sub>B))" 
       by blast
-    with ES stack_to_assembly_correct obtain \<Sigma>\<^sub>B' where SB': 
-      "\<Sigma>\<^sub>B' \<in> StackToAssembly.state_convert \<Sigma>\<^sub>S' \<and> iterate (eval_b_assembly ?\<Pi>\<^sub>B) \<Sigma>\<^sub>B \<Sigma>\<^sub>B'" by blast
+    with ES stack_to_assembly_correct flattening_correct obtain \<Sigma>\<^sub>B' where SB': 
+      "\<Sigma>\<^sub>B' \<in> StackToAssembly.state_convert (Flattening.state_convert \<Sigma>\<^sub>S') \<and> 
+        iterate (eval_b_assembly ?\<Pi>\<^sub>B) \<Sigma>\<^sub>B \<Sigma>\<^sub>B'" by blast
     with ES DA B debranching_correct have SA': "iterate (eval_assembly ?\<Pi>\<^sub>A)
       (Debranching.state_convert (dom ?\<Pi>\<^sub>B) \<Sigma>\<^sub>B) (Debranching.state_convert (dom ?\<Pi>\<^sub>B) \<Sigma>\<^sub>B')" by blast
     with DF linearization_correct have SL': "iterate (eval_l_assembly (linearize ?\<Pi>\<^sub>A)) 
@@ -58,7 +64,7 @@ theorem total_correctness: "finite (dom \<Pi>) \<Longrightarrow> iterate (eval_s
         (Linearization.state_convert (Debranching.state_convert (dom ?\<Pi>\<^sub>B) \<Sigma>\<^sub>B')) \<and> 
           iterate (eval_machine ?\<Pi>\<^sub>M) \<Sigma>\<^sub>M \<Sigma>\<^sub>M'" by blast
     with SA' SB' have "\<Sigma>\<^sub>M' \<in> { \<Sigma>\<^sub>M' | \<Sigma>\<^sub>B' \<Sigma>\<^sub>M'. 
-      \<Sigma>\<^sub>B' \<in> StackToAssembly.state_convert \<Sigma>\<^sub>S' \<and> 
+      \<Sigma>\<^sub>B' \<in> StackToAssembly.state_convert (Flattening.state_convert \<Sigma>\<^sub>S') \<and> 
         \<Sigma>\<^sub>M' \<in> AssemblyToMachine.state_convert (linearize ?\<Pi>\<^sub>A) 
           (Linearization.state_convert (Debranching.state_convert (dom ?\<Pi>\<^sub>B) \<Sigma>\<^sub>B')) }" 
       by blast
