Utilities/BasicComputation.thy
@@ -10,7 +10,7 @@ axiomatization new_label :: "code_label set \<Rightarrow> code_label" where
 type_synonym "output" = "int list"
 
 definition boolify :: "int \<Rightarrow> bool" where
-  "boolify i = (i = 0)"
+  "boolify i = (i \<noteq> 0)"
 
 definition unboolify :: "bool \<Rightarrow> int" where
   "unboolify b = (if b then 1 else 0)"
@@ -20,6 +20,9 @@ lemma [simp]: "unboolify True = 1"
 
 lemma [simp]: "unboolify False = 0"
   by (simp add: unboolify_def)
+
+lemma [simp]: "boolify (unboolify b) = b"
+  by (cases b) (simp_all add: boolify_def)
 
 lemma [simp]: "unboolify (boolify i2 \<and> boolify i1) = unboolify (boolify i1 \<and> boolify i2)"
   by (simp add: boolify_def unboolify_def)
