FlatStack/FlatStackLanguage.thy
@@ -1,0 +1,35 @@
+theory FlatStackLanguage
+imports "../Utilities/BasicComputation"
+begin
+
+datatype flat_stack_instruction = 
+  FAdd | FSub | FNeg | FEq | FGt | FLt | FAnd | FOr | FNot
+| FPrint
+
+type_synonym flat_stack_program = "code_label \<rightharpoonup> flat_stack_instruction list \<times> code_label"
+
+type_synonym flat_stack_state = "int list \<times> flat_stack_instruction list \<times> code_label \<times> output" 
+  (* \<sigma>, \<pi>, s, \<omega> *)
+
+fun eval_flat_stack :: "flat_stack_program \<Rightarrow> flat_stack_state \<Rightarrow> flat_stack_state option" where
+  "eval_flat_stack \<Pi> (\<sigma>, [], s, \<omega>) = (case \<Pi> s of
+      Some (\<pi>, s') \<Rightarrow> Some (\<sigma>, \<pi>, s', \<omega>)
+    | None \<Rightarrow> None)"
+| "eval_flat_stack \<Pi> (i1 # i2 # \<sigma>, FAdd # \<pi>, s, \<omega>) = Some ((i2 + i1) # \<sigma>, \<pi>, s, \<omega>)"
+| "eval_flat_stack \<Pi> (i1 # i2 # \<sigma>, FSub # \<pi>, s, \<omega>) = Some ((i2 - i1) # \<sigma>, \<pi>, s, \<omega>)"
+| "eval_flat_stack \<Pi> (i1 # \<sigma>, FNeg # \<pi>, s, \<omega>) = Some ((-i1) # \<sigma>, \<pi>, s, \<omega>)"
+| "eval_flat_stack \<Pi> (i1 # i2 # \<sigma>, FEq # \<pi>, s, \<omega>) = Some (unboolify (i2 = i1) # \<sigma>, \<pi>, s, \<omega>)"
+| "eval_flat_stack \<Pi> (i1 # i2 # \<sigma>, FGt # \<pi>, s, \<omega>) = Some (unboolify (i2 > i1) # \<sigma>, \<pi>, s, \<omega>)"
+| "eval_flat_stack \<Pi> (i1 # i2 # \<sigma>, FLt # \<pi>, s, \<omega>) = Some (unboolify (i2 < i1) # \<sigma>, \<pi>, s, \<omega>)"
+| "eval_flat_stack \<Pi> (i1 # i2 # \<sigma>, FAnd # \<pi>, s, \<omega>) = 
+    Some (unboolify (boolify i2 \<and> boolify i1) # \<sigma>, \<pi>, s, \<omega>)"
+| "eval_flat_stack \<Pi> (i1 # i2 # \<sigma>, FOr # \<pi>, s, \<omega>) = 
+    Some (unboolify (boolify i2 \<or> boolify i1) # \<sigma>, \<pi>, s, \<omega>)"
+| "eval_flat_stack \<Pi> (i1 # \<sigma>, FNot # \<pi>, s, \<omega>) = Some (unboolify (\<not> boolify i1) # \<sigma>, \<pi>, s, \<omega>)"
+| "eval_flat_stack \<Pi> (i1 # \<sigma>, FPrint # \<pi>, s, \<omega>) = Some (\<sigma>, \<pi>, s, i1 # \<omega>)"
+| "eval_flat_stack \<Pi> \<Sigma> = None"
+
+fun flat_stack_output :: "flat_stack_state \<Rightarrow> output" where
+  "flat_stack_output (\<sigma>, \<pi>, s, \<omega>) = \<omega>"
+
+end
